generalize CopyBuffer, ProbeActions

lib/everparse/3d/EverParse3d.CopyBuffer.fsti
@@ -1,15 +1,19 @@
 module EverParse3d.CopyBuffer
 module AppCtxt = EverParse3d.AppCtxt
-module I = EverParse3d.InputStream.All
+module I = EverParse3d.InputStream.Base
 module U8 = FStar.UInt8
 module U16 = FStar.UInt16
 module U32 = FStar.UInt32
 module U64 = FStar.UInt64
 open Pulse.Lib.Pervasives
 
-val copy_buffer_t : Type0
+class copy_buffer (copy_buffer_t: Type0) (input_buffer_t: Type0) {| I.input_stream_inst input_buffer_t |} = {
+  stream_of : copy_buffer_t -> input_buffer_t;
+}
 
-val stream_of : copy_buffer_t -> I.t
-
-let pts_to (c: copy_buffer_t) (contents: Seq.seq U8.t) (v: Seq.seq U8.t) : Tot slprop =
-  I.pts_to (stream_of c) contents v
+let pts_to
+  (#copy_buffer_t #input_buffer_t: Type0)
+  {| I.input_stream_inst input_buffer_t |}
+  {| copy_buffer copy_buffer_t input_buffer_t |}
+  (c: copy_buffer_t) (contents: Seq.seq U8.t) (v: Seq.seq U8.t) : Tot slprop =
+  I.pts_to #input_buffer_t (stream_of c) contents v
