lib/everparse/3d/EverParse3d.ProbeActions.fst
@@ -1,7 +1,12 @@
 module EverParse3d.ProbeActions
 #lang-pulse
 
-let probe_fn_incremental = 
+let probe_fn_incremental
+  (#copy_buffer_t: Type0)
+  (#input_buffer_t: Type0)
+  {| inst: I.input_stream_inst input_buffer_t  |}
+  {| cb_inst: copy_buffer copy_buffer_t input_buffer_t  |}
+= 
   bytes_to_read:U64.t ->
   read_offset:U64.t ->
   write_offset:U64.t ->
@@ -10,9 +15,9 @@ let probe_fn_incremental =
   contents_dest: Ghost.erased (Seq.seq U8.t) ->
   v_dest: Ghost.erased (Seq.seq U8.t) ->
   stt bool
-    (CB.pts_to dest contents_dest v_dest)
+    (CB.pts_to #_ #input_buffer_t dest contents_dest v_dest)
     (fun b -> exists* contents_dest' v_dest' .
-      CB.pts_to dest contents_dest v_dest **
+      CB.pts_to #_ #input_buffer_t dest contents_dest v_dest **
       pure
       (if b
        then (
@@ -27,29 +32,39 @@ let probe_fn_incremental =
 
 inline_for_extraction
 noextract
-let init_probe_dest_t =
+let init_probe_dest_t
+  (#copy_buffer_t: Type0)
+  (#input_buffer_t: Type0)
+  {| inst: I.input_stream_inst input_buffer_t  |}
+  {| cb_inst: copy_buffer copy_buffer_t input_buffer_t  |}
+=
   struct_name:string ->
   sz:U64.t ->
   dest:copy_buffer_t ->
   stt bool
     (exists* contents_dest v_dest .
-      CB.pts_to dest contents_dest v_dest
+      CB.pts_to #_ #input_buffer_t dest contents_dest v_dest
     )
     (fun b -> exists* contents_dest' .
-      CB.pts_to dest contents_dest' contents_dest'
+      CB.pts_to #_ #input_buffer_t dest contents_dest' contents_dest'
     )
 
 inline_for_extraction
-let write_at_offset_t (t:Type0) (n:U64.t) =
+let write_at_offset_t
+  (#copy_buffer_t: Type0)
+  (#input_buffer_t: Type0)
+  {| inst: I.input_stream_inst input_buffer_t  |}
+  {| cb_inst: copy_buffer copy_buffer_t input_buffer_t  |}
+(t:Type0) (n:U64.t) =
   v:t ->
   write_offset:U64.t ->
   dest:copy_buffer_t ->
   contents_dest: Ghost.erased (Seq.seq U8.t) ->
   v_dest: Ghost.erased (Seq.seq U8.t) ->
   stt bool
-    (CB.pts_to dest contents_dest v_dest)
+    (CB.pts_to #_ #input_buffer_t dest contents_dest v_dest)
     (fun b -> exists* contents_dest' v_dest' .
-      CB.pts_to dest contents_dest v_dest **
+      CB.pts_to #_ #input_buffer_t dest contents_dest v_dest **
       pure
       (if b
        then (
@@ -66,7 +81,12 @@ let coerce_value_t (t0 t1:Type0) = t0 -> t1
 
 inline_for_extraction
 noextract
-let probe_and_read_at_offset_t (t:Type0) (size_t:U64.t) =
+let probe_and_read_at_offset_t
+  (#copy_buffer_t: Type0)
+  (#input_buffer_t: Type0)
+  {| inst: I.input_stream_inst input_buffer_t  |}
+  {| cb_inst: copy_buffer copy_buffer_t input_buffer_t  |}
+  (t:Type0) (size_t:U64.t) =
   failed:ref bool ->
   read_offset:U64.t ->
   src:U64.t ->
@@ -74,11 +94,11 @@ let probe_and_read_at_offset_t (t:Type0) (size_t:U64.t) =
   stt t
     (exists* contents_dest v_dest .
       pts_to failed false **
-      CB.pts_to dest contents_dest v_dest
+      CB.pts_to #_ #input_buffer_t dest contents_dest v_dest
     )
     (fun _ -> exists* has_failed contents_dest' v_dest' .
       pts_to failed has_failed **
-      CB.pts_to dest contents_dest' v_dest' **
+      CB.pts_to #_ #input_buffer_t dest contents_dest' v_dest' **
       pure (
         not has_failed ==> U64.fits (U64.v read_offset + U64.v size_t)
       ))
@@ -117,8 +137,10 @@ let probe_m_post
 
 inline_for_extraction
 let probe_m
+  (#copy_buffer_t: Type0)
   (#input_buffer_t: Type0)
   {| inst: I.input_stream_inst input_buffer_t  |}
+  {| cb_inst: copy_buffer copy_buffer_t input_buffer_t  |}
   a (requires_unread_dest:bool) (expect_zero_offsets:bool) (use_error_handler:bool) =
   typename:string ->
   fieldname:string ->
@@ -139,7 +161,7 @@ let probe_m
       pts_to failed v_failed **
       pts_to read_offset v_read_offset **
       pts_to write_offset v_write_offset **
-      CB.pts_to dest contents_dest v_dest **
+      CB.pts_to #_ #input_buffer_t #_ #cb_inst dest contents_dest v_dest **
       pure
     (probe_m_pre
       requires_unread_dest expect_zero_offsets v_read_offset v_write_offset v_failed contents_dest v_dest)
@@ -149,7 +171,7 @@ let probe_m
       pts_to failed v_failed' **
       pts_to read_offset v_read_offset' **
       pts_to write_offset v_write_offset' **
-      CB.pts_to dest contents_dest' v_dest' **
+      CB.pts_to #_ #input_buffer_t #_ #cb_inst dest contents_dest' v_dest' **
       pure
     (probe_m_post
       v_read_offset v_read_offset' v_write_offset v_write_offset' contents_dest' v_dest')
@@ -165,8 +187,10 @@ let probe_m
 inline_for_extraction
 noextract
 fn handle_probe_error
+  (#copy_buffer_t: Type0)
   (#input_buffer_t: Type0)
   {| inst: I.input_stream_inst input_buffer_t  |}
+  {| cb_inst: copy_buffer copy_buffer_t input_buffer_t  |}
       (#use_error_handler:bool)
       (err : (if use_error_handler then error_handler #input_buffer_t else unit))
       (tn fn_ det:string)
@@ -175,10 +199,10 @@ fn handle_probe_error
       (contents_dest v_dest: Ghost.erased (Seq.seq U8.t))
 requires exists* v_ctxt .
       pts_to ctxt v_ctxt **
-      CB.pts_to dest contents_dest v_dest
+      CB.pts_to #_ #input_buffer_t dest contents_dest v_dest
 ensures exists* v_ctxt' .
       pts_to ctxt v_ctxt' **
-      CB.pts_to dest contents_dest v_dest
+      CB.pts_to #_ #input_buffer_t dest contents_dest v_dest
 {
   if (use_error_handler) {
 //    coerce_eq #_ #error_handler () err tn fn_ det 0uL ctxt (stream_of dest) 0uL _
@@ -192,10 +216,12 @@ ensures exists* v_ctxt' .
 inline_for_extraction
 noextract
 fn probe_fn_incremental_as_probe_m
+  (#copy_buffer_t: Type0)
   (#input_buffer_t: Type0)
   {| inst: I.input_stream_inst input_buffer_t  |}
-  (#use_error_handler:bool) (f:probe_fn_incremental) (bytes_to_read:U64.t)
-: probe_m #input_buffer_t unit true false use_error_handler
+  {| cb_inst: copy_buffer copy_buffer_t input_buffer_t  |}
+  (#use_error_handler:bool) (f:probe_fn_incremental #copy_buffer_t #input_buffer_t) (bytes_to_read:U64.t)
+: probe_m #copy_buffer_t #input_buffer_t unit true false use_error_handler
 =
   (tn: _)
   (fn_: _)
@@ -225,10 +251,12 @@ fn probe_fn_incremental_as_probe_m
 inline_for_extraction
 noextract
 let init_probe_m
+  (#copy_buffer_t: Type0)
   (#input_buffer_t: Type0)
   {| inst: I.input_stream_inst input_buffer_t  |}
+  {| cb_inst: copy_buffer copy_buffer_t input_buffer_t  |}
   (#use_error_handler:bool) struct_name (f:init_probe_dest_t)
-: probe_m unit false false use_error_handler
+: probe_m #copy_buffer_t #input_buffer_t unit false false use_error_handler
 = admit ()
 
 (*
@@ -244,10 +272,12 @@ fun _ _ _ ctxt err read_offset write_offset failed src sz dest ->
 inline_for_extraction
 noextract
 let init_probe_size
+  (#copy_buffer_t: Type0)
   (#input_buffer_t: Type0)
   {| inst: I.input_stream_inst input_buffer_t  |}
+  {| cb_inst: copy_buffer copy_buffer_t input_buffer_t  |}
   (#use_error_handler:bool)
-: probe_m U64.t true false use_error_handler
+: probe_m #copy_buffer_t #input_buffer_t U64.t true false use_error_handler
 = admit ()
 (*
 = fun _ _ _ ctxt err read_offset write_offset failed src sz dest ->
@@ -257,8 +287,10 @@ let init_probe_size
 inline_for_extraction
 noextract
 let write_at_offset_m
+  (#copy_buffer_t: Type0)
   (#input_buffer_t: Type0)
   {| inst: I.input_stream_inst input_buffer_t  |}
+  {| cb_inst: copy_buffer copy_buffer_t input_buffer_t  |}
   (#use_error_handler:bool) (#t:Type0) (#w:U64.t { w <> 0uL }) (f:write_at_offset_t t w) (v:t)
 : probe_m unit true false use_error_handler
 = admit ()
@@ -278,8 +310,10 @@ let write_at_offset_m
 inline_for_extraction
 noextract
 let probe_and_read_at_offset_m
+  (#copy_buffer_t: Type0)
   (#input_buffer_t: Type0)
   {| inst: I.input_stream_inst input_buffer_t  |}
+  {| cb_inst: copy_buffer copy_buffer_t input_buffer_t  |}
   (#use_error_handler:bool) (#t:Type0) (#s:U64.t { s <> 0uL }) (reader:probe_and_read_at_offset_t t s)
 : probe_m t true false use_error_handler
 = admit ()
@@ -302,8 +336,10 @@ let probe_and_read_at_offset_m
 inline_for_extraction
 noextract
 let seq_probe_m
+  (#copy_buffer_t: Type0)
   (#input_buffer_t: Type0)
   {| inst: I.input_stream_inst input_buffer_t  |}
+  {| cb_inst: copy_buffer copy_buffer_t input_buffer_t  |}
   (#use_error_handler:bool) (#a:Type) (detail:string) (dflt:a) (m1:probe_m unit true false use_error_handler) (m2:probe_m a true false use_error_handler)
 : probe_m a true false use_error_handler
 = admit ()
@@ -323,8 +359,10 @@ let seq_probe_m
 inline_for_extraction
 noextract
 let bind_probe_m
+  (#copy_buffer_t: Type0)
   (#input_buffer_t: Type0)
   {| inst: I.input_stream_inst input_buffer_t  |}
+  {| cb_inst: copy_buffer copy_buffer_t input_buffer_t  |}
   (#use_error_handler:bool) (#a #b:Type) (detail:string) (dflt:b) (m1:probe_m a true false use_error_handler) (m2:a -> probe_m b true false use_error_handler)
 : probe_m b true false use_error_handler
 = admit ()
@@ -343,8 +381,10 @@ let bind_probe_m
 inline_for_extraction
 noextract
 let probe_and_copy_init_sz
+  (#copy_buffer_t: Type0)
   (#input_buffer_t: Type0)
   {| inst: I.input_stream_inst input_buffer_t  |}
+  {| cb_inst: copy_buffer copy_buffer_t input_buffer_t  |}
   (#use_error_handler:bool) (f:probe_fn_incremental)
 : probe_m unit true false use_error_handler
 = bind_probe_m 
@@ -356,8 +396,10 @@ let probe_and_copy_init_sz
 inline_for_extraction
 noextract
 let return_probe_m
+  (#copy_buffer_t: Type0)
   (#input_buffer_t: Type0)
   {| inst: I.input_stream_inst input_buffer_t  |}
+  {| cb_inst: copy_buffer copy_buffer_t input_buffer_t  |}
   (#use_error_handler:bool) (#a:Type) (v:a)
 : probe_m a true false use_error_handler
 = admit ()
@@ -374,8 +416,10 @@ let check_overflow_add (x:U64.t) (y:U64.t)
 inline_for_extraction
 noextract
 let skip_read
+  (#copy_buffer_t: Type0)
   (#input_buffer_t: Type0)
   {| inst: I.input_stream_inst input_buffer_t  |}
+  {| cb_inst: copy_buffer copy_buffer_t input_buffer_t  |}
   (#use_error_handler:bool) (bytes_to_skip:U64.t)
 : probe_m unit true false use_error_handler
 = admit ()
@@ -394,8 +438,10 @@ let skip_read
 inline_for_extraction
 noextract
 let skip_write
+  (#copy_buffer_t: Type0)
   (#input_buffer_t: Type0)
   {| inst: I.input_stream_inst input_buffer_t  |}
+  {| cb_inst: copy_buffer copy_buffer_t input_buffer_t  |}
   (#use_error_handler:bool) (bytes_to_skip:U64.t)
 : probe_m unit true false use_error_handler
 = admit ()
@@ -414,8 +460,10 @@ let skip_write
 inline_for_extraction
 noextract
 let fail
+  (#copy_buffer_t: Type0)
   (#input_buffer_t: Type0)
   {| inst: I.input_stream_inst input_buffer_t  |}
+  {| cb_inst: copy_buffer copy_buffer_t input_buffer_t  |}
   (#use_error_handler:bool)
 : probe_m unit true false use_error_handler
 = admit ()
@@ -427,8 +475,10 @@ let fail
 inline_for_extraction
 noextract
 let if_then_else
+  (#copy_buffer_t: Type0)
   (#input_buffer_t: Type0)
   {| inst: I.input_stream_inst input_buffer_t  |}
+  {| cb_inst: copy_buffer copy_buffer_t input_buffer_t  |}
 (#use_error_handler:bool) (b:bool) (m0 m1:probe_m unit true false use_error_handler)
 : probe_m unit true false use_error_handler
 = admit ()
@@ -587,8 +637,10 @@ let probe_array_aux (#use_error_handler:bool) (byte_len:U64.t) (probe_elem:probe
 inline_for_extraction
 noextract
 let probe_array
+  (#copy_buffer_t: Type0)
   (#input_buffer_t: Type0)
   {| inst: I.input_stream_inst input_buffer_t  |}
+  {| cb_inst: copy_buffer copy_buffer_t input_buffer_t  |}
   (#use_error_handler:bool) (byte_len:U64.t) (probe_elem:probe_m unit true false use_error_handler)
 : probe_m unit true false use_error_handler
 = admit ()
@@ -599,8 +651,10 @@ let probe_array
 inline_for_extraction
 noextract
 let lift_pure_external_action
+  (#copy_buffer_t: Type0)
   (#input_buffer_t: Type0)
   {| inst: I.input_stream_inst input_buffer_t  |}
+  {| cb_inst: copy_buffer copy_buffer_t input_buffer_t  |}
   (#use_error_handler:bool) (#a:Type) (f:pure_external_action a)
 : probe_m a true false use_error_handler
 = admit ()
@@ -611,8 +665,10 @@ let lift_pure_external_action
 inline_for_extraction
 noextract
 let init_and_probe
+  (#copy_buffer_t: Type0)
   (#input_buffer_t: Type0)
   {| inst: I.input_stream_inst input_buffer_t  |}
+  {| cb_inst: copy_buffer copy_buffer_t input_buffer_t  |}
       (#use_error_handler:bool)
       (#mz:bool)
       (struct_name:string)
