lib/everparse/3d/EverParse3d.ProbeActions.fsti
@@ -13,139 +13,215 @@ open EverParse3d.Actions.Common
 
 inline_for_extraction
 noextract
-val probe_fn_incremental : Type0
+val probe_fn_incremental
+  (#copy_buffer_t: Type0)
+  (#input_buffer_t: Type0)
+  {| inst: I.input_stream_inst input_buffer_t  |}
+  {| cb_inst: copy_buffer copy_buffer_t input_buffer_t  |}
+: Type0
 
 inline_for_extraction
 noextract
-val init_probe_dest_t : Type0
+val init_probe_dest_t
+  (#copy_buffer_t: Type0)
+  (#input_buffer_t: Type0)
+  {| inst: I.input_stream_inst input_buffer_t  |}
+  {| cb_inst: copy_buffer copy_buffer_t input_buffer_t  |}
+: Type0
 
 inline_for_extraction
-val write_at_offset_t (t:Type0) (n:U64.t) : Type0
+val write_at_offset_t
+  (#copy_buffer_t: Type0)
+  (#input_buffer_t: Type0)
+  {| inst: I.input_stream_inst input_buffer_t  |}
+  {| cb_inst: copy_buffer copy_buffer_t input_buffer_t  |}
+  (t:Type0) (n:U64.t) : Type0
 
 inline_for_extraction
 noextract
-val probe_and_read_at_offset_t (t:Type0) (size_t:U64.t) : Type0
+val probe_and_read_at_offset_t
+  (#copy_buffer_t: Type0)
+  (#input_buffer_t: Type0)
+  {| inst: I.input_stream_inst input_buffer_t  |}
+  {| cb_inst: copy_buffer copy_buffer_t input_buffer_t  |}
+(t:Type0) (size_t:U64.t) : Type0
 
 inline_for_extraction
-let probe_and_read_at_offset_uint8 = probe_and_read_at_offset_t U8.t 1uL
+let probe_and_read_at_offset_uint8
+  (#copy_buffer_t: Type0)
+  (#input_buffer_t: Type0)
+  {| inst: I.input_stream_inst input_buffer_t  |}
+  {| cb_inst: copy_buffer copy_buffer_t input_buffer_t  |}
+= probe_and_read_at_offset_t #copy_buffer_t #input_buffer_t U8.t 1uL
 inline_for_extraction
-let probe_and_read_at_offset_uint16 = probe_and_read_at_offset_t U16.t 2uL
+let probe_and_read_at_offset_uint16
+  (#copy_buffer_t: Type0)
+  (#input_buffer_t: Type0)
+  {| inst: I.input_stream_inst input_buffer_t  |}
+  {| cb_inst: copy_buffer copy_buffer_t input_buffer_t  |}
+= probe_and_read_at_offset_t #copy_buffer_t #input_buffer_t U16.t 2uL
 inline_for_extraction
-let probe_and_read_at_offset_uint32 = probe_and_read_at_offset_t U32.t 4uL
+let probe_and_read_at_offset_uint32
+  (#copy_buffer_t: Type0)
+  (#input_buffer_t: Type0)
+  {| inst: I.input_stream_inst input_buffer_t  |}
+  {| cb_inst: copy_buffer copy_buffer_t input_buffer_t  |}
+= probe_and_read_at_offset_t #copy_buffer_t #input_buffer_t U32.t 4uL
 inline_for_extraction
-let probe_and_read_at_offset_uint64 = probe_and_read_at_offset_t U64.t 8uL
+let probe_and_read_at_offset_uint64
+  (#copy_buffer_t: Type0)
+  (#input_buffer_t: Type0)
+  {| inst: I.input_stream_inst input_buffer_t  |}
+  {| cb_inst: copy_buffer copy_buffer_t input_buffer_t  |}
+= probe_and_read_at_offset_t #copy_buffer_t #input_buffer_t U64.t 8uL
 inline_for_extraction
-let write_at_offset_uint8 = write_at_offset_t U8.t 1uL
+let write_at_offset_uint8
+  (#copy_buffer_t: Type0)
+  (#input_buffer_t: Type0)
+  {| inst: I.input_stream_inst input_buffer_t  |}
+  {| cb_inst: copy_buffer copy_buffer_t input_buffer_t  |}
+= write_at_offset_t #copy_buffer_t #input_buffer_t U8.t 1uL
 inline_for_extraction
-let write_at_offset_uint16 = write_at_offset_t U16.t 2uL
+let write_at_offset_uint16
+  (#copy_buffer_t: Type0)
+  (#input_buffer_t: Type0)
+  {| inst: I.input_stream_inst input_buffer_t  |}
+  {| cb_inst: copy_buffer copy_buffer_t input_buffer_t  |}
+= write_at_offset_t #copy_buffer_t #input_buffer_t U16.t 2uL
 inline_for_extraction
-let write_at_offset_uint32 = write_at_offset_t U32.t 4uL
+let write_at_offset_uint32
+  (#copy_buffer_t: Type0)
+  (#input_buffer_t: Type0)
+  {| inst: I.input_stream_inst input_buffer_t  |}
+  {| cb_inst: copy_buffer copy_buffer_t input_buffer_t  |}
+= write_at_offset_t #copy_buffer_t #input_buffer_t U32.t 4uL
 inline_for_extraction
-let write_at_offset_uint64 = write_at_offset_t U64.t 8uL
+let write_at_offset_uint64
+  (#copy_buffer_t: Type0)
+  (#input_buffer_t: Type0)
+  {| inst: I.input_stream_inst input_buffer_t  |}
+  {| cb_inst: copy_buffer copy_buffer_t input_buffer_t  |}
+= write_at_offset_t #copy_buffer_t #input_buffer_t U64.t 8uL
 
 inline_for_extraction
 val probe_m
+  (#copy_buffer_t: Type0)
   (#input_buffer_t: Type0)
   {| inst: I.input_stream_inst input_buffer_t  |}
+  {| cb_inst: copy_buffer copy_buffer_t input_buffer_t  |}
   (a:Type0) (requires_unread_dest:bool) (expect_zero_offsets:bool) (use_error_handler:bool) : Type0
 
 inline_for_extraction
 noextract
 val probe_fn_incremental_as_probe_m
   {| inst: I.input_stream_inst 'input_buffer_t  |}
-(#use_error_handler:bool) (f:probe_fn_incremental) (bytes_to_read:U64.t)
-: probe_m #_ #inst unit true false use_error_handler
+  {| cbinst: copy_buffer 'copy_buffer_t 'input_buffer_t |}
+(#use_error_handler:bool) (f:probe_fn_incremental #'copy_buffer_t #'input_buffer_t) (bytes_to_read:U64.t)
+: probe_m #_ #_ #inst #cbinst unit true false use_error_handler
 
 inline_for_extraction
 noextract
 val init_probe_m
   {| inst: I.input_stream_inst 'input_buffer_t  |}
-(#use_error_handler:bool) (probe_struct_name:string) (f:init_probe_dest_t)
-: probe_m #_ #inst unit false false use_error_handler
+  {| cbinst: copy_buffer 'copy_buffer_t 'input_buffer_t |}
+(#use_error_handler:bool) (probe_struct_name:string) (f:init_probe_dest_t #'copy_buffer_t #'input_buffer_t)
+: probe_m #_ #_ #inst #cbinst unit false false use_error_handler
 
 inline_for_extraction
 noextract
 val init_probe_size
   {| inst: I.input_stream_inst 'input_buffer_t  |}
+  {| cbinst: copy_buffer 'copy_buffer_t 'input_buffer_t |}
   (#use_error_handler:bool)
-: probe_m #_ #inst U64.t true false use_error_handler
+: probe_m #_ #_ #inst #cbinst U64.t true false use_error_handler
 
 inline_for_extraction
 noextract
 val write_at_offset_m
   {| inst: I.input_stream_inst 'input_buffer_t  |}
-  (#use_error_handler:bool) (#t:Type0) (#w:U64.t { w <> 0uL }) (f:write_at_offset_t t w) (v:t)
-: probe_m #_ #inst unit true false use_error_handler
+  {| cbinst: copy_buffer 'copy_buffer_t 'input_buffer_t |}
+  (#use_error_handler:bool) (#t:Type0) (#w:U64.t { w <> 0uL }) (f:write_at_offset_t #'copy_buffer_t #'input_buffer_t t w) (v:t)
+: probe_m #_ #_ #inst #cbinst unit true false use_error_handler
 
 inline_for_extraction
 noextract
 val probe_and_read_at_offset_m
   {| inst: I.input_stream_inst 'input_buffer_t  |}
-  (#use_error_handler:bool) (#t:Type0) (#s:U64.t { s <> 0uL }) (reader:probe_and_read_at_offset_t t s)
-: probe_m #_ #inst t true false use_error_handler
+  {| cbinst: copy_buffer 'copy_buffer_t 'input_buffer_t |}
+  (#use_error_handler:bool) (#t:Type0) (#s:U64.t { s <> 0uL }) (reader:probe_and_read_at_offset_t #'copy_buffer_t #'input_buffer_t t s)
+: probe_m #_ #_ #inst #cbinst t true false use_error_handler
 
 inline_for_extraction
 noextract
 val seq_probe_m
   {| inst: I.input_stream_inst 'input_buffer_t  |}
-  (#use_error_handler:bool) (#a:Type) (detail:string) (dflt:a) (m1:probe_m #_ #inst unit true false use_error_handler) (m2:probe_m #_ #inst a true false use_error_handler)
-: probe_m #_ #inst a true false use_error_handler
+  {| cbinst: copy_buffer 'copy_buffer_t 'input_buffer_t |}
+  (#use_error_handler:bool) (#a:Type) (detail:string) (dflt:a) (m1:probe_m #_ #_ #inst #cbinst unit true false use_error_handler) (m2:probe_m #_ #_ #inst #cbinst a true false use_error_handler)
+: probe_m #_ #_ #inst #cbinst a true false use_error_handler
 
 inline_for_extraction
 noextract
 val bind_probe_m
   {| inst: I.input_stream_inst 'input_buffer_t  |}
-  (#use_error_handler:bool) (#a #b:Type) (detail:string) (dflt:b) (m1:probe_m #_ #inst a true false use_error_handler) (m2:a -> probe_m #_ #inst b true false use_error_handler)
-: probe_m #_ #inst b true false use_error_handler
+  {| cbinst: copy_buffer 'copy_buffer_t 'input_buffer_t |}
+  (#use_error_handler:bool) (#a #b:Type) (detail:string) (dflt:b) (m1:probe_m #_ #_ #inst #cbinst a true false use_error_handler) (m2:a -> probe_m #_ #_ #inst #cbinst b true false use_error_handler)
+: probe_m #_ #_ #inst #cbinst b true false use_error_handler
 
 inline_for_extraction
 noextract
 val probe_and_copy_init_sz
   {| inst: I.input_stream_inst 'input_buffer_t  |}
-  (#use_error_handler:bool) (f:probe_fn_incremental)
-: probe_m #_ #inst unit true false use_error_handler
+  {| cbinst: copy_buffer 'copy_buffer_t 'input_buffer_t |}
+  (#use_error_handler:bool) (f:probe_fn_incremental #'copy_buffer_t #'input_buffer_t)
+: probe_m #_ #_ #inst #cbinst unit true false use_error_handler
 
 inline_for_extraction
 noextract
 val return_probe_m
   {| inst: I.input_stream_inst 'input_buffer_t  |}
+  {| cbinst: copy_buffer 'copy_buffer_t 'input_buffer_t |}
   (#use_error_handler:bool) (#a:Type) (v:a)
-: probe_m #_ #inst a true false use_error_handler
+: probe_m #_ #_ #inst #cbinst a true false use_error_handler
 
 inline_for_extraction
 noextract
 val skip_read
   {| inst: I.input_stream_inst 'input_buffer_t  |}
+  {| cbinst: copy_buffer 'copy_buffer_t 'input_buffer_t |}
   (#use_error_handler:bool) (bytes_to_skip:U64.t)
-: probe_m #_ #inst unit true false use_error_handler
+: probe_m #_ #_ #inst #cbinst unit true false use_error_handler
 
 inline_for_extraction
 noextract
 val skip_write
   {| inst: I.input_stream_inst 'input_buffer_t  |}
+  {| cbinst: copy_buffer 'copy_buffer_t 'input_buffer_t |}
   (#use_error_handler:bool) (bytes_to_skip:U64.t)
-: probe_m #_ #inst unit true false use_error_handler
+: probe_m #_ #_ #inst #cbinst unit true false use_error_handler
 
 inline_for_extraction
 noextract
 val fail
   {| inst: I.input_stream_inst 'input_buffer_t  |}
+  {| cbinst: copy_buffer 'copy_buffer_t 'input_buffer_t |}
   (#use_error_handler:bool)
-: probe_m #_ #inst unit true false use_error_handler
+: probe_m #_ #_ #inst #cbinst unit true false use_error_handler
 
 inline_for_extraction
 noextract
 val if_then_else
   {| inst: I.input_stream_inst 'input_buffer_t  |}
-  (#use_error_handler:bool) (b:bool) (m0 m1:probe_m #_ #inst unit true false use_error_handler)
-: probe_m #_ #inst unit true false use_error_handler
+  {| cbinst: copy_buffer 'copy_buffer_t 'input_buffer_t |}
+  (#use_error_handler:bool) (b:bool) (m0 m1:probe_m #_ #_ #inst #cbinst unit true false use_error_handler)
+: probe_m #_ #_ #inst #cbinst unit true false use_error_handler
 
 inline_for_extraction
 noextract
 val probe_array
   {| inst: I.input_stream_inst 'input_buffer_t  |}
-  (#use_error_handler:bool) (byte_len:U64.t) (probe_elem:probe_m #_ #inst unit true false use_error_handler)
-: probe_m #_ #inst unit true false use_error_handler
+  {| cbinst: copy_buffer 'copy_buffer_t 'input_buffer_t |}
+  (#use_error_handler:bool) (byte_len:U64.t) (probe_elem:probe_m #_ #_ #inst #cbinst unit true false use_error_handler)
+: probe_m #_ #_ #inst #cbinst unit true false use_error_handler
 
 inline_for_extraction
 noextract
@@ -156,39 +232,42 @@ inline_for_extraction
 noextract
 val lift_pure_external_action
   {| inst: I.input_stream_inst 'input_buffer_t  |}
+  {| cbinst: copy_buffer 'copy_buffer_t 'input_buffer_t |}
   (#use_error_handler:bool) (#a:Type) (f:pure_external_action a)
-: probe_m #_ #inst a true false use_error_handler
+: probe_m #_ #_ #inst #cbinst a true false use_error_handler
 
 inline_for_extraction
 noextract
 val init_and_probe 
   {| inst: I.input_stream_inst 'input_buffer_t  |}
+  {| cbinst: copy_buffer 'copy_buffer_t 'input_buffer_t |}
       (#use_error_handler:bool)
       (#mz:bool)
       (struct_name:string)
-      (init:init_probe_dest_t)
-      (probe:probe_m #_ #inst unit true mz use_error_handler)
-: probe_m #_ #inst unit false mz use_error_handler
+      (init:init_probe_dest_t #'copy_buffer_t #'input_buffer_t)
+      (probe:probe_m #_ #_ #inst #cbinst unit true mz use_error_handler)
+: probe_m #_ #_ #inst #cbinst unit false mz use_error_handler
 
 inline_for_extraction
 noextract
 val run_probe_m
   {| inst: I.input_stream_inst 'input_buffer_t  |}
+  {| cb_inst: copy_buffer 'copy_buffer_t 'input_buffer_t  |}
   (#use_error_handler:bool) (#any:bool) 
-  (m:probe_m #_ #inst unit false any use_error_handler)
+  (m:probe_m #_ #_ #inst #cb_inst unit false any use_error_handler)
   (tn fn det:string)
   (ctxt:app_ctxt)
   (err:(if use_error_handler then error_handler #_ #inst else unit))
   (src:U64.t)
   (sz:U64.t)
-  (dest:copy_buffer_t)
+  (dest:'copy_buffer_t)
 : stt U64.t
     (exists* v_ctxt contents_dest v_dest .
       pts_to ctxt v_ctxt **
-      CB.pts_to dest contents_dest v_dest
+      CB.pts_to #_ #_ #_ #cb_inst dest contents_dest v_dest
     )
     (fun b -> exists* v_ctxt' contents_dest' v_dest' .
       pts_to ctxt v_ctxt' **
-      CB.pts_to dest contents_dest' v_dest' **
+      CB.pts_to #_ #_ #_ #cb_inst dest contents_dest' v_dest' **
       pure (b <> 0uL ==> contents_dest' == v_dest')
     )
